Adding exps for Poly

proof/Poly/Exp.v
@@ -1,13 +1,80 @@
 
 Require Import Ty.
+Require Import Env.
 Require Import Base.
 
 
 (** Expressions *****************************************************)
 Inductive exp : Type :=
  | XVar  : nat -> exp
+ | XLAM  : exp -> exp
+ | XAPP  : exp -> exp -> exp
  | XLam  : ty  -> exp -> exp
  | XApp  : exp -> exp -> exp.
 Hint Constructors exp.
+
+
+(* Closedness *******************************************************)
+
+(* Exp is val closed under a type environment of a given length *)
+Inductive coversXX : nat -> exp -> Prop :=
+ | CoversXX_var
+   :  forall n i
+   ,  n > i
+   -> coversXX n (XVar i)
+
+ | CoversXX_LAM
+   :  forall n x
+   ,  coversXX (S n) x
+   -> coversXX n (XLAM x)
+
+ | CoversXX_APP 
+   :  forall n x t
+   ,  coversXX n t
+   -> coversXX n (XAPP x t)
+
+ | CoversXX_lam
+   :  forall n t x
+   ,  coversXX n x
+   -> coversXX n (XLam t x)
+
+ | CoversXX_app
+   :  forall n x1 x2
+   ,  coversXX n x1 -> coversXX n x2
+   -> coversXX n (XApp x1 x2).
+Hint Constructors coversXX.
+
+
+(* Exp is val closed under the given type environment *)
+Inductive closedUnderXX : tyenv -> exp -> Prop :=
+  |  ClosedUnderXX 
+     :  forall tenv x
+     ,  coversXX (length tenv) x
+     -> closedUnderXX tenv x.
+Hint Constructors closedUnderXX.
+
+
+(* Exp is val closed under the empty type environment *)
+Inductive closedXX : exp -> Prop :=
+ |  ClosedXX
+    :  forall x
+    ,  coversXX 0 x
+    -> closedXX x.
+Hint Constructors closedXX.
+
+
+(* Lemmas ***********************************************************)
+Lemma coversXX_succ
+ :  forall n x
+ ,  coversXX n     x
+ -> coversXX (S n) x.
+Proof.
+ intros. gen n.
+ induction x; intros; inversions H; auto.
+Qed.
+Hint Resolve coversT_succ.
+
+
+
 
 
